Test/dafny0/Corecursion.dfy
@@ -9,7 +9,7 @@ module CoRecursion {
     More(n, AscendingChain(n+1))
   }
 
-  function AscendingChainAndRead(n: int): Stream<int>
+  function AscendingChainAndRead(n: nat): Stream<int>
     reads this;  // with a reads clause, this function is not a co-recusvie function
   {
     More(n, AscendingChainAndRead(n+1))  // error: cannot prove termination
